switch to more translator-friendly version of pmatch
uses all_envs throughout, uses write, doesn't do type-checking, doesn't
bother with the store. still calls lookup_alist_mod_env directly: not
sure if that should be through some other interface...

pmatch/testScript.sml
@@ -13,38 +13,169 @@ val EvalPatRel_def = Define`
         [(p,(Lit(Unit)))] ARB
         ((0,empty_store),if ∃vars. pat vars = x then Rval(Litv(Unit)) else Rerr(Rraise ARB))`
 
-(* want version of pmatch that doesn't break apart an all_env, but does bindings with write *)
+(*
+val Pmatch_def = tDefine"Pmatch"`
+  (Pmatch env [] [] = Match env) ∧
+  (Pmatch env (p1::p2::ps) (v1::v2::vs) =
+     case Pmatch env [p1] [v1] of
+     | No_match => No_match
+     | Match_type_error => Match_type_error
+     | Match env' => Pmatch env' (p2::ps) (v2::vs)) ∧
+  (Pmatch env [Pvar x] [v] = Match (write x v env)) ∧
+  (Pmatch env [Plit l] [Litv l'] =
+     if l = l' then Match env
+     else if lit_same_type l l' then No_match
+     else Match_type_error) ∧
+  (Pmatch env [Pcon (SOME n) ps] [Conv (SOME (n',t')) vs] =
+     case lookup_alist_mod_env n (all_env_to_cenv env) of
+     | SOME (l,t) =>
+       if same_tid t t' ∧ LENGTH ps = l then
+         if same_ctor (id_to_n n, t) (n',t') then
+           Pmatch env ps vs
+         else No_match
+       else Match_type_error
+     | _ => Match_type_error) ∧
+  (Pmatch env [Pcon NONE ps] [Conv NONE vs] =
+     if LENGTH ps = LENGTH vs then
+       Pmatch env ps vs
+     else Match_type_error) ∧
+  (Pmatch env [Pref p] [Loc lnum] =
+     Match_type_error)`
+(WF_REL_TAC`measure (pat1_size o FST o SND)`)
+*)
+
+val Pmatch_def = tDefine"Pmatch"`
+  (Pmatch env [] [] = SOME env) ∧
+  (Pmatch env (p1::p2::ps) (v1::v2::vs) =
+     case Pmatch env [p1] [v1] of | NONE => NONE
+     | SOME env' => Pmatch env' (p2::ps) (v2::vs)) ∧
+  (Pmatch env [Pvar x] [v] = SOME (write x v env)) ∧
+  (Pmatch env [Plit l] [Litv l'] =
+     if l = l' then SOME env else NONE) ∧
+  (Pmatch env [Pcon (SOME n) ps] [Conv (SOME (n',t')) vs] =
+     case lookup_alist_mod_env n (all_env_to_cenv env) of | NONE => NONE
+     | SOME (l,t) =>
+       if same_tid t t' ∧ LENGTH ps = l ∧ same_ctor (id_to_n n, t) (n',t') then
+           Pmatch env ps vs
+       else NONE) ∧
+  (Pmatch env [Pcon NONE ps] [Conv NONE vs] =
+     if LENGTH ps = LENGTH vs then
+       Pmatch env ps vs
+     else NONE) ∧
+  (Pmatch env _ _ = NONE)`
+(WF_REL_TAC`measure (pat1_size o FST o SND)`)
+
+val Pmatch_ind = theorem"Pmatch_ind"
+
 val EvalPatBind_def = Define`
   EvalPatBind env a p pat vars env2 ⇔
-    ∃x av enve.
+    ∃x av.
       a x av ∧
-      pmatch (all_env_to_cenv env) empty_store p av (all_env_to_env env) = Match enve ∧
-      (env2 = (all_env_to_menv env,all_env_to_cenv env,enve)) ∧
+      (Pmatch env [p] [av] = SOME env2) ∧
       (pat vars = x)`
+
+val Pmatch_cons = store_thm("Pmatch_cons",
+  ``∀ps vs.
+      Pmatch env (p::ps) (v::vs) =
+      case Pmatch env [p] [v] of | NONE => NONE
+      | SOME env' => Pmatch env' ps vs``,
+  Induct >> Cases_on`vs` >> simp[Pmatch_def] >>
+  BasicProvers.CASE_TAC >>
+  Cases_on`ps`>>simp[Pmatch_def])
+
+val Pmatch_SOME_const = store_thm("Pmatch_SOME_const",
+  ``∀env ps vs env'.
+      Pmatch env ps vs = SOME env' ⇒
+      all_env_to_menv env' = all_env_to_menv env ∧
+      all_env_to_cenv env' = all_env_to_cenv env``,
+  ho_match_mp_tac Pmatch_ind >> simp[Pmatch_def] >>
+  rw[] >> BasicProvers.EVERY_CASE_TAC >> fs[] >>
+  PairCases_on`env`>>
+  fs[write_def,all_env_to_cenv_def,all_env_to_menv_def])
+
+val pmatch_imp_Pmatch = prove(
+  ``(∀envC s p v env.
+      s = empty_store ⇒
+      case pmatch envC s p v env of
+      | Match env' =>
+        Pmatch (envM,envC,env) [p] [v] = SOME (envM,envC,env')
+      | _ => Pmatch (envM,envC,env) [p] [v] = NONE) ∧
+    (∀envC s ps vs env.
+      s = empty_store ⇒
+      case pmatch_list envC s ps vs env of
+      | Match env' =>
+        Pmatch (envM,envC,env) ps vs = SOME (envM,envC,env')
+      | _ => Pmatch (envM,envC,env) ps vs = NONE)``,
+  ho_match_mp_tac pmatch_ind >>
+  rw[pmatch_def,Pmatch_def,write_def,all_env_to_cenv_def]
+  >- (
+    BasicProvers.CASE_TAC >>
+    BasicProvers.CASE_TAC >>
+    BasicProvers.CASE_TAC >> fs[] >>
+    BasicProvers.CASE_TAC >> fs[] )
+  >- (
+    BasicProvers.CASE_TAC >>
+    BasicProvers.CASE_TAC >>
+    BasicProvers.CASE_TAC >>
+    fs[store_lookup_def] >>
+    fs[empty_store_def])
+  >- (
+    BasicProvers.CASE_TAC >> fs[] >>
+    simp[Once Pmatch_cons] >>
+    BasicProvers.CASE_TAC >> fs[] >>
+    simp[Once Pmatch_cons] )
+  >- (
+    Cases_on`v110`>>simp[Pmatch_def]))
+  |> SIMP_RULE std_ss []
+  |> curry save_thm "pmatch_imp_Pmatch"
+
+val Pmatch_imp_pmatch = store_thm("Pmatch_imp_pmatch",
+  ``∀env ps vs env'.
+      (Pmatch env ps vs = SOME env' ⇒
+       pmatch_list (all_env_to_cenv env) empty_store ps vs (all_env_to_env env) =
+         Match (all_env_to_env env')) ∧
+      (Pmatch env ps vs = NONE ⇒
+       ∀env2.
+       pmatch_list (all_env_to_cenv env) empty_store ps vs (all_env_to_env env) ≠
+         Match env2)``,
+  ho_match_mp_tac Pmatch_ind >>
+  simp[Pmatch_def,pmatch_def] >> rw[] >>
+  `∃envM envC envE. env = (envM,envC,envE)` by METIS_TAC[PAIR] >>
+  fs[all_env_to_cenv_def,all_env_to_menv_def,all_env_to_env_def,write_def] >>
+  BasicProvers.CASE_TAC >> fs[] >>
+  BasicProvers.EVERY_CASE_TAC >> rfs[] >> rw[] >>
+  imp_res_tac Pmatch_SOME_const >>
+  fs[all_env_to_cenv_def,all_env_to_menv_def,all_env_to_env_def,write_def] >>
+  rfs[] >>
+  Cases_on`v20`>>fs[pmatch_def] >>
+  BasicProvers.EVERY_CASE_TAC >> fs[store_lookup_def,empty_store_def])
 
 val pmatch_PMATCH_ROW_COND_No_match = store_thm("pmatch_PMATCH_ROW_COND_No_match",
   ``EvalPatRel env a p pat ∧
     (∀vars. ¬PMATCH_ROW_COND pat (K T) xv vars) ∧
     a xv res ⇒
-    pmatch (all_env_to_cenv env) empty_store p res (all_env_to_env env) = No_match``,
+    Pmatch env [p] [res] = NONE``,
   rw[EvalPatRel_def] >>
   first_x_assum(fn th => first_x_assum(strip_assume_tac o MATCH_MP th)) >>
-  fs[Eval_def,Once evaluate_cases] >>
-  `∃menv cenv eenv. env = (menv,cenv,eenv)` by METIS_TAC[PAIR] >> fs[] >>
-  simp[all_env_to_cenv_def,all_env_to_env_def] >> fs[write_def] >>
-  fs[Once evaluate_cases,lookup_var_id_def] >>
-  rfs[PMATCH_ROW_COND_def])
+  `∃envM envC envE. env = (envM,envC,envE)` by METIS_TAC[PAIR] >> fs[] >>
+  qspecl_then[`envC`,`p`,`res`,`envE`]strip_assume_tac(CONJUNCT1 pmatch_imp_Pmatch) >>
+  fs[Eval_def,Once evaluate_cases] >> rfs[] >>
+  rpt(pop_assum mp_tac) >>
+  rw[Once evaluate_cases,PMATCH_ROW_COND_def])
 
 val pmatch_PMATCH_ROW_COND_Match = store_thm("pmatch_PMATCH_ROW_COND_Match",
   ``EvalPatRel env a p pat ∧
     PMATCH_ROW_COND pat (K T) xv vars ∧
     a xv res
-    ⇒ ∃env2. pmatch (all_env_to_cenv env) empty_store p res (all_env_to_env env) = Match env2``,
+    ⇒ ∃env2. Pmatch env [p] [res] = SOME env2``,
   rw[EvalPatRel_def,PMATCH_ROW_COND_def] >>
   first_x_assum(fn th => first_x_assum(strip_assume_tac o MATCH_MP th)) >>
-  fs[Once evaluate_cases,all_env_to_cenv_def,all_env_to_env_def] >>
+  `∃envM envC envE. env = (envM,envC,envE)` by METIS_TAC[PAIR] >> fs[] >>
+  qspecl_then[`envC`,`p`,`res`,`envE`]strip_assume_tac(CONJUNCT1 pmatch_imp_Pmatch) >>
+  fs[Once evaluate_cases] >> rfs[] >>
+  BasicProvers.EVERY_CASE_TAC >> fs[] >>
   fs[Once evaluate_cases] >>
-  BasicProvers.EVERY_CASE_TAC >> fs[] >> PROVE_TAC[])
+  PROVE_TAC[])
 
 val Eval_PMATCH_NIL = store_thm("Eval_PMATCH_NIL",
   ``CONTAINER F ⇒
@@ -79,7 +210,10 @@ val Eval_PMATCH = store_thm("Eval_PMATCH",
     first_x_assum(qspec_then`vars`mp_tac)>>simp[] >> strip_tac >>
     first_x_assum(fn th => first_assum(strip_assume_tac o MATCH_MP th)) >>
     srw_tac[DNF_ss][] >> disj1_tac >>
-    fs[all_env_to_cenv_def,all_env_to_env_def] >>
+    imp_res_tac Pmatch_imp_pmatch >>
+    imp_res_tac Pmatch_SOME_const >>
+    fs[all_env_to_cenv_def,all_env_to_env_def,pmatch_def,all_env_to_menv_def] >>
+    qpat_assum`X = Match Y` mp_tac >> BasicProvers.CASE_TAC >>
     fs[GSYM AND_IMP_INTRO] >>
     first_x_assum(fn th => first_assum(strip_assume_tac o MATCH_MP th)) >>
     rfs[] >>
@@ -88,7 +222,8 @@ val Eval_PMATCH = store_thm("Eval_PMATCH",
     `(some x. pat x = pat vars) = SOME vars` by (
       simp[optionTheory.some_def] >>
       METIS_TAC[] ) >>
-    simp[] >> fs[all_env_to_menv_def] >>
+    simp[] >> fs[all_env_to_menv_def] >> rw[] >>
+    PairCases_on`env2`>> fs[all_env_to_cenv_def,all_env_to_env_def,pmatch_def,all_env_to_menv_def] >>
     METIS_TAC[]) >>
   qpat_assum`evaluate F X Y (Mat A B) R`mp_tac >>
   simp[Once evaluate_cases] >> strip_tac >>
@@ -96,8 +231,12 @@ val Eval_PMATCH = store_thm("Eval_PMATCH",
   srw_tac[DNF_ss][] >> disj2_tac >>
   simp[PMATCH_def,PMATCH_ROW_def] >>
   imp_res_tac pmatch_PMATCH_ROW_COND_No_match >>
-  fs[all_env_to_cenv_def,all_env_to_env_def] >>
-  METIS_TAC[])
+  imp_res_tac Pmatch_imp_pmatch >>
+  fs[all_env_to_cenv_def,all_env_to_env_def,pmatch_def] >>
+  pop_assum mp_tac >> BasicProvers.CASE_TAC >- METIS_TAC[] >>
+  fs[EvalPatRel_def] >>
+  first_x_assum(fn th => first_x_assum(mp_tac o MATCH_MP th)) >>
+  simp[Once evaluate_cases] >> rw[])
 
 val () = set_trace"use pmatch_pp"0
 val () = register_type``:'a list``
@@ -188,11 +327,11 @@ val gth2 = TAC_PROOF((asms,gtm2),
   simp[EvalPatBind_def,all_env_to_cenv_def,all_env_to_env_def,PULL_EXISTS,all_env_to_menv_def] >>
   simp[UNCURRY,LIST_TYPE_def,PULL_EXISTS] >>
   fs[lookup_cons_def] >>
-  simp[pmatch_def,same_tid_def,same_ctor_def,id_to_n_def] >>
+  simp[Pmatch_def,all_env_to_cenv_def,same_tid_def,same_ctor_def,id_to_n_def] >>
   simp[Eval_def] >>
   simp[Once evaluate_cases,PULL_EXISTS] >>
   simp[Once evaluate_cases,PULL_EXISTS] >>
-  simp[Once evaluate_cases,PULL_EXISTS,lookup_var_id_def] >>
+  simp[Once evaluate_cases,PULL_EXISTS,lookup_var_id_def,write_def] >>
   simp[Once evaluate_cases,PULL_EXISTS] >>
   simp[Once evaluate_cases,PULL_EXISTS] >>
   simp[Once evaluate_cases,PULL_EXISTS] >>
